examples/AKE/AKE_proof.ec
@@ -5,10 +5,11 @@ require import FSet.
 require import List.
 require import Fun.
 require import Real.
+require import Pair.
 
 require import AKE_defs.
 
-(*{ Initial game and security definition *)
+(*{ AKE: Initial game and security definition *)
 
 (* The initial module: we keep it simple and inline the
    definitions of h1 and h2. *)
@@ -29,6 +30,21 @@ module AKE(FA : Adv) = {
   var mStarted   : (Sidx, Sdata) map  (* map of started sessions *)
   var mCompleted : (Sidx, Epk)   map  (* additional data for completed sessions *)
   
+  fun init() : unit = {
+    evs = [];
+    test = None;
+    cSession = 0;
+    cH1 = 0;
+    cH2 = 0;
+    mH1 = Map.empty;
+    sH1 = FSet.empty;
+    mH2 = Map.empty;
+    sH2 = FSet.empty;
+    mSk = Map.empty;
+    mStarted = Map.empty;
+    mCompleted = Map.empty;
+  }
+
   module O : AKE_Oracles = {
 
     fun h1(a : Sk, x : Esk) : Eexp = {
@@ -170,29 +186,19 @@ module AKE(FA : Adv) = {
     var t_idx : Sidx = def;
     var key : Key = def;
     var keyo : Key option = def;
-    var b' : bool = false = def;
+    var b' : bool = def;
     var i : int = 0;
     var ska : Sk = def;
     var pka : Pk = def;
 
-    mSk = Map.empty;
+    init();
+
     while (i < qAgent) {
       ska = $sample_Sk;
       pka = gen_pk(ska);
       pks = pka :: pks;
       mSk.[pka] = ska;
     } 
-    cSession = 0;
-    cH1 = 0;
-    cH2 = 0;
-    mH1 = Map.empty;
-    sH1 = FSet.empty;
-    mH2 = Map.empty;
-    sH2 = FSet.empty;
-    mStarted = Map.empty;
-    mCompleted = Map.empty;
-    evs = [];
-    test = None;
 
     t_idx = A.choose(pks);
     b = ${0,1};
@@ -228,7 +234,7 @@ end section.
 
 (*} end: Initial game and security definition *)
 
-(*{ First reduction: replace H1_A by EexpRev oracle *)
+(*{ First reduction: AKE_EexpRev (replace H1_A by EexpRev oracle) *)
 
 module type AKE_Oracles2 = {
   fun eexpRev(i : Sidx, a : Sk) : Eexp option
@@ -390,7 +396,7 @@ module AKE_EexpRev(FA : Adv2) = {
     var ska : Sk = def;
     var pka : Pk = def;
     var xa' : Eexp = def;
-
+    
     mSk = Map.empty;
     while (i < qAgent) {
       ska = $sample_Sk;
@@ -454,3 +460,503 @@ section.
 end section.
 
 (*} *)
+
+(*{ Proof: Pr[ AKE : win ] <= eps + Pr[ AKE_EexpRev : win ] *)
+
+op esk_of_sidx (mStarted : (Sidx, Sdata) map) (i : Sidx) =
+  sd_esk(proj mStarted.[i]).
+
+op esks(mStarted : (Sidx, Sdata) map) : Esk set =
+  img sd_esk (frng mStarted).
+
+print op fdom.
+
+op queried_esks(mH1 : ((Sk * Esk), Eexp)  map) : Esk set =
+  img snd (fdom mH1).
+
+(* Introduce bad flags for collision events *)
+module AKE_1(FA : Adv) = {
+  
+  var evs  : Event list               (* events for queries performed by adversary *)
+  var test : Sid option               (* session id of test session *)
+
+  var cSession, cH1, cH2 : int        (* counters for queries *)
+
+  var mH1 : ((Sk * Esk), Eexp) map    (* map for h1 *)
+  var sH1 : (Sk * Esk) set            (* adversary queries for h1 *)
+
+  var mH2 : (Sstring, Key) map        (* map for h2 *)
+  var sH2 : Sstring set               (* adversary queries for h2 *)
+
+  var mSk        : (Agent, Sk) map    (* map for static secret keys *)
+  var mStarted   : (Sidx, Sdata) map  (* map of started sessions *)
+  var mCompleted : (Sidx, Epk)   map  (* additional data for completed sessions *)
+
+  var bad_esk_col : bool              (* esk collision with dom(mH1) *)
+    (* The esk sampled in init1/resp is already in dom(mH1). Since
+       dom(mH1) = sH1 u <earlier esks>, this corresponds to
+       esk-earlier-esk collisions and esk-earlier-h1_a collisions *)
+
+  var bad_esk_norev : bool            (* h1_a query without previous reveal *)
+  
+
+  fun init() : unit = {
+    evs = [];
+    test = None;
+    cSession = 0;
+    cH1 = 0;
+    cH2 = 0;
+    mH1 = Map.empty;
+    sH1 = FSet.empty;
+    mH2 = Map.empty;
+    sH2 = FSet.empty;
+    mSk = Map.empty;
+    mStarted = Map.empty;
+    mCompleted = Map.empty;
+    bad_esk_col = false;
+    bad_esk_norev = false;
+  }
+
+  module O : AKE_Oracles = {
+
+    fun h1(a : Sk, x : Esk) : Eexp = {
+      var e : Eexp;
+      e = $sample_Eexp;
+      if (!in_dom (a,x) mH1) {
+        cH1 = cH1 + 1;
+        mH1.[(a,x)] = e;
+      } 
+      return proj mH1.[(a,x)];
+    }
+
+    fun h1_a(a : Sk, x : Esk) : Eexp option = {
+      var r : Eexp option = None;
+      var xe : Eexp;
+      if (cH1 < qH1) {
+        cH1 = cH1 + 1;
+        if (any (lambda i, let sd = proj mStarted.[i] in
+                           sd_esk sd = x /\
+                           ! (mem (EphemeralRev (psid_of_sdata sd)) evs))
+                (fdom mStarted)) {
+          bad_esk_norev = true;
+        }
+        sH1 = add (a,x) sH1;
+        xe = h1(a,x);
+        r = Some(xe);
+      }
+      return r;
+    }
+
+    fun h2(sstring : Sstring) : Key = {
+      var ke : Key;
+      ke = $sample_Key;
+      if (!in_dom sstring mH2) {
+        mH2.[sstring] = ke;
+      }
+      return proj mH2.[sstring];
+    }
+ 
+    fun h2_a(sstring : Sstring) : Key option = {
+      var r : Key option = None;
+      var ks : Key;
+      if (cH2 < qH2) {
+        cH2 = cH2 + 1;
+        sH2 = add sstring sH2;
+        ks = h2(sstring);
+        r = Some(ks);
+      }
+      return r;
+    }
+
+    fun init1(i : Sidx, A : Agent, B : Agent) : Epk option = {
+      var x : Esk;
+      var x' : Eexp;
+      var pX : Epk;
+      var r : Epk option = None; 
+      if (cSession < qSession && in_dom A mSk && in_dom B mSk && !in_dom i mStarted) {
+        cSession = cSession + 1;
+        x  = $sample_Esk;
+        if (mem x (queried_esks mH1)) bad_esk_col = true;
+        x' = h1(proj (mSk.[A]),x);
+        pX = gen_epk(x');
+        mStarted.[i] = (A,B,x,x',init);
+        r = Some(pX);
+        evs = Start(psid_of_sdata(proj mStarted.[i]))::evs;
+      }
+      return r;
+    }
+
+    fun resp(i : Sidx, B : Agent, A : Agent, X : Epk) : Epk option = {
+      var y : Esk;
+      var y' : Eexp;
+      var pY : Epk;
+      var r : Epk option = None; 
+      if (   cSession < qSession && in_dom A mSk && in_dom B mSk
+          && !in_dom i mStarted && !in_dom i mCompleted) {
+        cSession = cSession + 1;
+        y  = $sample_Esk;
+        if (mem y (queried_esks mH1)) bad_esk_col = true;
+        y' = h1(proj (mSk.[B]),y);
+        pY = gen_epk(y');
+        mStarted.[i] = (B,A,y,y',resp);
+        mCompleted.[i] = X;
+        r = Some(pY);
+        evs = Accept(sid_of_sdata (proj mStarted.[i]) X)::evs;
+      }
+      return r;
+    }
+
+    fun init2(i : Sidx, Y : Epk) : unit = {
+      if (!in_dom i mCompleted && in_dom i mStarted) {
+        mCompleted.[i] = Y;
+        evs = Accept(sid_of_sdata(proj mStarted.[i]) Y)::evs;
+      }
+    }
+
+    fun staticRev(A : Agent) : Sk option = {
+      var r : Sk option = None;
+      if (in_dom A mSk) {
+        r = mSk.[A];
+        evs = StaticRev(A)::evs;
+      }
+      return r;
+    }
+
+    fun ephemeralRev(i : Sidx) : Esk option = {
+      var r : Esk option = None;
+      if (in_dom i mStarted) {
+        r = Some(sd_esk(proj mStarted.[i]));
+        evs = EphemeralRev(psid_of_sdata(proj mStarted.[i]))::evs;
+      }
+      return r;
+    }
+
+    fun computeKey(i : Sidx) : Key option = {
+      var rv : Key option = None;
+      var a, b : Agent;
+      var r : Role;
+      var x' : Eexp;
+      var x : Esk;
+      var key : Key;
+      if (in_dom i mCompleted) {
+        (a,b,x,x',r) = proj mStarted.[i];
+        key = h2(gen_sstring x' (proj mSk.[a]) b (proj mCompleted.[i]) r);
+        rv = Some key;
+      }
+      return rv;
+    }
+
+    fun sessionRev(i : Sidx) : Key option = {
+      var r : Key option = None;
+      var s : Sid;
+      if (in_dom i mCompleted) {
+        s = sid_of_sdata (proj mStarted.[i]) (proj mCompleted.[i]);
+        evs = SessionRev(sid_of_sdata(proj mStarted.[i]) (proj mCompleted.[i]))::evs;
+        r = computeKey(i);
+      }
+      return r;
+    }
+  }
+  
+  module A = FA(O)
+
+  fun main() : bool = {
+    var b : bool = def;
+    var pks : Pk list = [];
+    var t_idx : Sidx = def;
+    var key : Key = def;
+    var keyo : Key option = def;
+    var b' : bool = def;
+    var i : int = 0;
+    var ska : Sk = def;
+    var pka : Pk = def;
+
+    init();
+    while (i < qAgent) {
+      ska = $sample_Sk;
+      pka = gen_pk(ska);
+      pks = pka :: pks;
+      mSk.[pka] = ska;
+    } 
+
+    t_idx = A.choose(pks);
+    b = ${0,1};
+    if (mStarted.[t_idx] <> None && mCompleted.[t_idx] <> None) {
+      test = Some (sid_of_sdata (proj mStarted.[t_idx]) (proj mCompleted.[t_idx]));
+        (* the if-condition implies "mem (Accept (proj O.test)) O.evs" *)
+      if (b) {
+        keyo = O.computeKey(t_idx);
+      } else {
+        key  = $sample_Key;
+        keyo = Some key;
+      }
+      b' = A.guess(keyo);
+    }
+    return (b = b');
+  }
+}.
+
+lemma Eq_AKE_AKE_1(A <: Adv{AKE, AKE_1}):
+  equiv[ AKE(A).main ~ AKE_1(A).main : true ==>
+            (res /\ test_fresh AKE.test AKE.evs){1}
+         => (res /\ test_fresh AKE_1.test AKE_1.evs){2}].
+proof strict.
+  (* Simulate forward proof manually for which automated proof should be possible *)
+  fun.
+  seq 10 10: (* we would do this step by step and add variables to the post *)
+    (={b,pks,t_idx,key,keyo,b',i,ska,pka} /\
+     AKE.mSk{1}        = AKE_1.mSk{2} /\
+     AKE.cSession{1}   = AKE_1.cSession{2} /\
+     AKE.cH1{1}        = AKE_1.cH1{2} /\
+     AKE.cH2{1}        = AKE_1.cH2{2} /\
+     AKE.mH1{1}        = AKE_1.mH1{2} /\
+     AKE.sH1{1}        = AKE_1.sH1{2} /\
+     AKE.mH2{1}        = AKE_1.mH2{2} /\
+     AKE.sH2{1}        = AKE_1.sH2{2} /\
+     AKE.mStarted{1}   = AKE_1.mStarted{2} /\
+     AKE.mCompleted{1} = AKE_1.mCompleted{2} /\
+     AKE.evs{1}        = AKE_1.evs{2} /\
+     AKE.test{1}       = AKE_1.test{2}).
+  inline AKE(A).init AKE_1(A).init.
+  wp. trivial.
+  seq 1 1:
+    (={b,pks,t_idx,key,keyo,b',i,ska,pka} /\
+     AKE.mSk{1}        = AKE_1.mSk{2} /\
+     AKE.cSession{1}   = AKE_1.cSession{2} /\
+     AKE.cH1{1}        = AKE_1.cH1{2} /\
+     AKE.cH2{1}        = AKE_1.cH2{2} /\
+     AKE.mH1{1}        = AKE_1.mH1{2} /\
+     AKE.sH1{1}        = AKE_1.sH1{2} /\
+     AKE.mH2{1}        = AKE_1.mH2{2} /\
+     AKE.sH2{1}        = AKE_1.sH2{2} /\
+     AKE.mStarted{1}   = AKE_1.mStarted{2} /\
+     AKE.mCompleted{1} = AKE_1.mCompleted{2} /\
+     AKE.evs{1}        = AKE_1.evs{2} /\
+     AKE.test{1}       = AKE_1.test{2}).
+  eqobs_in. (* slow *) 
+  seq 1 1:
+    (={b,pks,t_idx,key,keyo,b',i,ska,pka} /\
+     AKE.mSk{1}        = AKE_1.mSk{2} /\
+     AKE.cSession{1}   = AKE_1.cSession{2} /\
+     AKE.cH1{1}        = AKE_1.cH1{2} /\
+     AKE.cH2{1}        = AKE_1.cH2{2} /\
+     AKE.mH1{1}        = AKE_1.mH1{2} /\
+     AKE.sH1{1}        = AKE_1.sH1{2} /\
+     AKE.mH2{1}        = AKE_1.mH2{2} /\
+     AKE.sH2{1}        = AKE_1.sH2{2} /\
+     AKE.mStarted{1}   = AKE_1.mStarted{2} /\
+     AKE.mCompleted{1} = AKE_1.mCompleted{2} /\
+     AKE.evs{1}        = AKE_1.evs{2} /\
+     AKE.test{1}       = AKE_1.test{2}).
+  eqobs_in. (* again slow *)
+  seq 1 1:
+    (={b,pks,t_idx,key,keyo,b',i,ska,pka} /\
+     AKE.mSk{1}        = AKE_1.mSk{2} /\
+     AKE.cSession{1}   = AKE_1.cSession{2} /\
+     AKE.cH1{1}        = AKE_1.cH1{2} /\
+     AKE.cH2{1}        = AKE_1.cH2{2} /\
+     AKE.mH1{1}        = AKE_1.mH1{2} /\
+     AKE.sH1{1}        = AKE_1.sH1{2} /\
+     AKE.mH2{1}        = AKE_1.mH2{2} /\
+     AKE.sH2{1}        = AKE_1.sH2{2} /\
+     AKE.mStarted{1}   = AKE_1.mStarted{2} /\
+     AKE.mCompleted{1} = AKE_1.mCompleted{2} /\
+     AKE.evs{1}        = AKE_1.evs{2} /\
+     AKE.test{1}       = AKE_1.test{2}).
+  rnd. skip. progress. (* slow *)
+  if; [ by progress | | by skip; progress ].
+  seq 2 2:
+    (={b,pks,t_idx,key,keyo,b',i,ska,pka} /\
+     AKE.mSk{1}        = AKE_1.mSk{2} /\
+     AKE.cSession{1}   = AKE_1.cSession{2} /\
+     AKE.cH1{1}        = AKE_1.cH1{2} /\
+     AKE.cH2{1}        = AKE_1.cH2{2} /\
+     AKE.mH1{1}        = AKE_1.mH1{2} /\
+     AKE.sH1{1}        = AKE_1.sH1{2} /\
+     AKE.mH2{1}        = AKE_1.mH2{2} /\
+     AKE.sH2{1}        = AKE_1.sH2{2} /\
+     AKE.mStarted{1}   = AKE_1.mStarted{2} /\
+     AKE.mCompleted{1} = AKE_1.mCompleted{2} /\
+     AKE.evs{1}        = AKE_1.evs{2} /\
+     AKE.test{1}       = AKE_1.test{2} /\
+     ={glob A}).
+  eqobs_in.
+  call (_:
+    (AKE.mSk{1}        = AKE_1.mSk{2} /\
+     AKE.cSession{1}   = AKE_1.cSession{2} /\
+     AKE.cH1{1}        = AKE_1.cH1{2} /\
+     AKE.cH2{1}        = AKE_1.cH2{2} /\
+     AKE.mH1{1}        = AKE_1.mH1{2} /\
+     AKE.sH1{1}        = AKE_1.sH1{2} /\
+     AKE.mH2{1}        = AKE_1.mH2{2} /\
+     AKE.sH2{1}        = AKE_1.sH2{2} /\
+     AKE.mStarted{1}   = AKE_1.mStarted{2} /\
+     AKE.mCompleted{1} = AKE_1.mCompleted{2} /\
+     AKE.evs{1}        = AKE_1.evs{2} /\
+     AKE.test{1}       = AKE_1.test{2})).
+  skip. progress.
+  seq 1 1:
+    (={b,pks,t_idx,key,keyo,b',i,ska,pka} /\
+     AKE.mSk{1}        = AKE_1.mSk{2} /\
+     AKE.cSession{1}   = AKE_1.cSession{2} /\
+     AKE.cH1{1}        = AKE_1.cH1{2} /\
+     AKE.cH2{1}        = AKE_1.cH2{2} /\
+     AKE.mH1{1}        = AKE_1.mH1{2} /\
+     AKE.sH1{1}        = AKE_1.sH1{2} /\
+     AKE.mH2{1}        = AKE_1.mH2{2} /\
+     AKE.sH2{1}        = AKE_1.sH2{2} /\
+     AKE.mStarted{1}   = AKE_1.mStarted{2} /\
+     AKE.mCompleted{1} = AKE_1.mCompleted{2} /\
+     AKE.evs{1}        = AKE_1.evs{2} /\
+     AKE.test{1}       = AKE_1.test{2} /\
+    ={glob A}).
+  rnd. skip. progress.
+  if; [ by progress| | skip; progress].
+  seq 1 1:
+    (={b,pks,t_idx,key,keyo,b',i,ska,pka} /\
+     AKE.mSk{1}        = AKE_1.mSk{2} /\
+     AKE.cSession{1}   = AKE_1.cSession{2} /\
+     AKE.cH1{1}        = AKE_1.cH1{2} /\
+     AKE.cH2{1}        = AKE_1.cH2{2} /\
+     AKE.mH1{1}        = AKE_1.mH1{2} /\
+     AKE.sH1{1}        = AKE_1.sH1{2} /\
+     AKE.mH2{1}        = AKE_1.mH2{2} /\
+     AKE.sH2{1}        = AKE_1.sH2{2} /\
+     AKE.mStarted{1}   = AKE_1.mStarted{2} /\
+     AKE.mCompleted{1} = AKE_1.mCompleted{2} /\
+     AKE.evs{1}        = AKE_1.evs{2} /\
+     AKE.test{1}       = AKE_1.test{2} /\
+    ={glob A}).
+  wp; skip; progress.
+  (* skip IF *)
+  seq 1 1:
+    (={b,pks,t_idx,key,keyo,b',i,ska,pka} /\
+     AKE.mSk{1}        = AKE_1.mSk{2} /\
+     AKE.cSession{1}   = AKE_1.cSession{2} /\
+     AKE.cH1{1}        = AKE_1.cH1{2} /\
+     AKE.cH2{1}        = AKE_1.cH2{2} /\
+     AKE.mH1{1}        = AKE_1.mH1{2} /\
+     AKE.sH1{1}        = AKE_1.sH1{2} /\
+     AKE.mH2{1}        = AKE_1.mH2{2} /\
+     AKE.sH2{1}        = AKE_1.sH2{2} /\
+     AKE.mStarted{1}   = AKE_1.mStarted{2} /\
+     AKE.mCompleted{1} = AKE_1.mCompleted{2} /\
+     AKE.evs{1}        = AKE_1.evs{2} /\
+     AKE.test{1}       = AKE_1.test{2} /\
+    ={glob A}).
+  if. progress.
+  call (_:
+    (AKE.mSk{1}        = AKE_1.mSk{2} /\
+     AKE.cSession{1}   = AKE_1.cSession{2} /\
+     AKE.cH1{1}        = AKE_1.cH1{2} /\
+     AKE.cH2{1}        = AKE_1.cH2{2} /\
+     AKE.mH1{1}        = AKE_1.mH1{2} /\
+     AKE.sH1{1}        = AKE_1.sH1{2} /\
+     AKE.mH2{1}        = AKE_1.mH2{2} /\
+     AKE.sH2{1}        = AKE_1.sH2{2} /\
+     AKE.mStarted{1}   = AKE_1.mStarted{2} /\
+     AKE.mCompleted{1} = AKE_1.mCompleted{2} /\
+     AKE.evs{1}        = AKE_1.evs{2} /\
+     AKE.test{1}       = AKE_1.test{2})).
+  eqobs_in. skip; progress.
+  wp. rnd. skip; progress.
+  call (_:
+    (AKE.mSk{1}        = AKE_1.mSk{2} /\
+     AKE.cSession{1}   = AKE_1.cSession{2} /\
+     AKE.cH1{1}        = AKE_1.cH1{2} /\
+     AKE.cH2{1}        = AKE_1.cH2{2} /\
+     AKE.mH1{1}        = AKE_1.mH1{2} /\
+     AKE.sH1{1}        = AKE_1.sH1{2} /\
+     AKE.mH2{1}        = AKE_1.mH2{2} /\
+     AKE.sH2{1}        = AKE_1.sH2{2} /\
+     AKE.mStarted{1}   = AKE_1.mStarted{2} /\
+     AKE.mCompleted{1} = AKE_1.mCompleted{2} /\
+     AKE.evs{1}        = AKE_1.evs{2} /\
+     AKE.test{1}       = AKE_1.test{2})).
+     
+     (* h1_a *)
+     fun. sp. if. progress. sp.
+     seq 1 1:
+      (={xe} /\
+       AKE.mSk{1}        = AKE_1.mSk{2} /\
+       AKE.cSession{1}   = AKE_1.cSession{2} /\
+       AKE.cH1{1}        = AKE_1.cH1{2} /\
+       AKE.cH2{1}        = AKE_1.cH2{2} /\
+       AKE.mH1{1}        = AKE_1.mH1{2} /\
+       AKE.sH1{1}        = AKE_1.sH1{2} /\
+       AKE.mH2{1}        = AKE_1.mH2{2} /\
+       AKE.sH2{1}        = AKE_1.sH2{2} /\
+       AKE.mStarted{1}   = AKE_1.mStarted{2} /\
+       AKE.mCompleted{1} = AKE_1.mCompleted{2} /\
+       AKE.evs{1}        = AKE_1.evs{2} /\
+       AKE.test{1}       = AKE_1.test{2}).
+       inline AKE_1(A).O.h1 AKE(A).O.h1.
+       eqobs_in. smt. wp. skip. smt. skip. smt.
+     (* h2_a *)
+     fun; eqobs_in.
+     (* init1 *)
+     fun. sp. if. progress.
+     wp.
+     seq 3 4:
+      (={i,x',x,A,B} /\
+       AKE.mSk{1}        = AKE_1.mSk{2} /\
+       AKE.cSession{1}   = AKE_1.cSession{2} /\
+       AKE.cH1{1}        = AKE_1.cH1{2} /\
+       AKE.cH2{1}        = AKE_1.cH2{2} /\
+       AKE.mH1{1}        = AKE_1.mH1{2} /\
+       AKE.sH1{1}        = AKE_1.sH1{2} /\
+       AKE.mH2{1}        = AKE_1.mH2{2} /\
+       AKE.sH2{1}        = AKE_1.sH2{2} /\
+       AKE.mStarted{1}   = AKE_1.mStarted{2} /\
+       AKE.mCompleted{1} = AKE_1.mCompleted{2} /\
+       AKE.evs{1}        = AKE_1.evs{2} /\
+       AKE.test{1}       = AKE_1.test{2}).
+       inline AKE_1(A).O.h1 AKE(A).O.h1.
+       eqobs_in. wp. rnd. wp.
+       skip. progress.
+     skip; progress. skip. progress.
+     (* init2 *)
+     fun; eqobs_in.
+     (* resp *)
+     fun. sp. if. progress.
+     wp.
+     seq 3 4:
+      (={i,y',y,X,A,B} /\
+       AKE.mSk{1}        = AKE_1.mSk{2} /\
+       AKE.cSession{1}   = AKE_1.cSession{2} /\
+       AKE.cH1{1}        = AKE_1.cH1{2} /\
+       AKE.cH2{1}        = AKE_1.cH2{2} /\
+       AKE.mH1{1}        = AKE_1.mH1{2} /\
+       AKE.sH1{1}        = AKE_1.sH1{2} /\
+       AKE.mH2{1}        = AKE_1.mH2{2} /\
+       AKE.sH2{1}        = AKE_1.sH2{2} /\
+       AKE.mStarted{1}   = AKE_1.mStarted{2} /\
+       AKE.mCompleted{1} = AKE_1.mCompleted{2} /\
+       AKE.evs{1}        = AKE_1.evs{2} /\
+       AKE.test{1}       = AKE_1.test{2}).
+       inline AKE_1(A).O.h1 AKE(A).O.h1.
+       eqobs_in. wp. rnd. wp.
+       skip. progress.
+     skip; progress. skip. progress.
+     (* staticRev *)
+     fun; eqobs_in.
+     (* ephemeralRev *)
+     fun; eqobs_in.
+     (* sessionRev *)
+     fun; eqobs_in.
+  skip. smt.
+qed. (* we only add ghost state, there should be an automated tactic *)
+
+lemma Pr_AKE_1_bad(A <: Adv) &m:
+       Pr[ AKE_1(A).main() @ &m : res /\ test_fresh AKE_1.test AKE_1.evs ]
+  <=   Pr[ AKE_1(A).main() @ &m : res /\ test_fresh AKE_1.test AKE_1.evs /\
+                                  !AKE_1.bad_esk_norev /\ !AKE_1.bad_esk_col]
+     + Pr[ AKE_1(A).main() @ &m : AKE_1.bad_esk_col ]
+     + Pr[ AKE_1(A).main() @ &m : (! AKE_1.bad_esk_col) /\ AKE_1.bad_esk_norev ].
+proof strict.
+  admit.
+qed.
+
+
+
+(*} end: Proof: Pr[ AKE : win ] <= eps + Pr[ AKE_EexpRev : win ] *)
